Token.v
@@ -43,3 +43,31 @@ Fixpoint lex (s : string) : list token :=
                    end
   | EmptyString => []
   end.
+
+Fixpoint to_string (ts : list token) : string :=
+  match ts with
+  | t :: ts' => String (to_ascii t) (to_string ts')
+  | [] => EmptyString
+  end.
+
+Fixpoint strip_comments (s : string) : string :=
+  match s with
+  | String a s' => match of_ascii a with
+                   | Some _ => String a (strip_comments s')
+                   | None => strip_comments s'
+                   end
+  | EmptyString => EmptyString
+  end.
+
+Ltac ascii_cases s :=
+  induction s as [| a s IHs];
+  [| destruct a as [[] [] [] [] [] [] [] []]; cbn; rewrite IHs];
+  reflexivity.
+
+Theorem strip_comments_lex : forall s,
+  lex (strip_comments s) = lex s.
+Proof. ascii_cases s. Qed.
+
+Theorem lex_to_string : forall s,
+  to_string (lex s) = strip_comments s.
+Proof. ascii_cases s. Qed.
